PhysLean/StringTheory/FTheory/SU5U1/Potential/ChargeProfile/Basic.lean
@@ -1,0 +1,435 @@
+/-
+Copyright (c) 2025 Joseph Tooby-Smith. All rights reserved.
+Released under Apache 2.0 license as described in the file LICENSE.
+Authors: Joseph Tooby-Smith
+-/
+import PhysLean.StringTheory.FTheory.SU5U1.Potential.Basic
+/-!
+
+# Charge profile
+
+The charge profile is a data structure which can be associated with each term of the potential.
+
+The charge profile is defined such that a given theory (that is specficication of
+`SU(5) × U(1)` representations) gives for each term of the potential `T` an element of
+`T.ChargeProfile`. This element specifies the possible values of charges
+one can assign to the fields present in `T`.
+
+For example for `T` the term `𝜆ᵢⱼₖ 5̄Mⁱ 5̄Mʲ 10ᵏ` the charge profile is `Finset ℤ × Finset ℤ`,
+and a theory with 3 `5̄M` fields of charges `{-3, 2, 1}` and 2 `10` fields of charges `{0, 1}`
+gives the charge profile `({-3, 2, 1}, {0, 1})` for this `T`.
+
+## Related PRs
+
+- See #562 for a first version of code related to charge profiles.
+
+-/
+
+namespace FTheory
+
+namespace SU5U1
+
+variable {I : CodimensionOneConfig}
+namespace PotentialTerm
+
+/-- The charge profiles of the potential terms in the `SU(5) × U(1)` theory.
+  This assigns to each potential term `T` a type `T.ChargeProfile`
+  which specifies the possible values of charges one can assign to the fields present in `T`.
+
+The types correspond to:
+- `μ` : `qHd × qHu`
+- `β` : `qHu × Q5`
+- `Λ` : `Q5 × Q10`
+- `W1` : `Q5 × Q10`
+- `W2` : `qHd × Q10`
+- `W3` : `qHu × Q5`
+- `W4` : `qHd × qHu × Q5`
+- `K1` : `Q5 × Q10`
+- `K2` : `qHd × qHu × Q10`
+- `topYukawa` : `qHu × Q10`
+- `bottomYukawa` : `qHd × Q5 × Q10`
+-/
+def ChargeProfile : PotentialTerm → Type
+    /- qHd × qHu -/
+  | μ => Option ℤ × Option ℤ
+  /- qHu × Q5 -/
+  | β => Option ℤ × Finset ℤ
+  /- Q5 × Q10 -/
+  | Λ => Finset ℤ × Finset ℤ
+  /- Q5 × Q10 -/
+  | W1 => Finset ℤ × Finset ℤ
+  /- qHd × Q10 -/
+  | W2 => Option ℤ × Finset ℤ
+  /- qHu × Q5 -/
+  | W3 => Option ℤ × Finset ℤ
+  /- qHd × qHu × Q5 -/
+  | W4 => Option ℤ × Option ℤ × Finset ℤ
+  /- Q5 × Q10 -/
+  | K1 => Finset ℤ × Finset ℤ
+  /- qHd × qHu × Q10 -/
+  | K2 => Option ℤ × Option ℤ × Finset ℤ
+  /- qHu × Q10 -/
+  | topYukawa => Option ℤ × Finset ℤ
+  /- qHd × Q5 × Q10 -/
+  | bottomYukawa => Option ℤ × Finset ℤ × Finset ℤ
+
+namespace ChargeProfile
+
+/-- For each term in the potential the charge profile is a decidable type. -/
+instance : (T : PotentialTerm) → DecidableEq T.ChargeProfile
+  | μ => inferInstanceAs (DecidableEq (Option ℤ × Option ℤ))
+  | β => inferInstanceAs (DecidableEq (Option ℤ × Finset ℤ))
+  | Λ => inferInstanceAs (DecidableEq (Finset ℤ × Finset ℤ))
+  | W1 => inferInstanceAs (DecidableEq (Finset ℤ × Finset ℤ))
+  | W2 => inferInstanceAs (DecidableEq (Option ℤ × Finset ℤ))
+  | W3 => inferInstanceAs (DecidableEq (Option ℤ × Finset ℤ))
+  | W4 => inferInstanceAs (DecidableEq (Option ℤ × Option ℤ × Finset ℤ))
+  | K1 => inferInstanceAs (DecidableEq (Finset ℤ × Finset ℤ))
+  | K2 => inferInstanceAs (DecidableEq (Option ℤ × Option ℤ × Finset ℤ))
+  | topYukawa => inferInstanceAs (DecidableEq (Option ℤ × Finset ℤ))
+  | bottomYukawa => inferInstanceAs (DecidableEq (Option ℤ × Finset ℤ × Finset ℤ))
+
+
+/-!
+
+## Subset relation on `ChargeProfile`
+
+For each charge profile, there is the subset relation.
+-/
+
+instance (T : PotentialTerm) : HasSubset T.ChargeProfile where Subset x y :=
+  match T with
+  | μ => x.1.toFinset ⊆ y.1.toFinset ∧ x.2.toFinset ⊆ y.2.toFinset
+  | β => x.1.toFinset ⊆ y.1.toFinset ∧ x.2 ⊆ y.2
+  | Λ => x.1 ⊆ y.1 ∧ x.2 ⊆ y.2
+  | W1 => x.1 ⊆ y.1 ∧ x.2 ⊆ y.2
+  | W2 => x.1.toFinset ⊆ y.1.toFinset ∧ x.2 ⊆ y.2
+  | W3 => x.1.toFinset ⊆ y.1.toFinset ∧ x.2 ⊆ y.2
+  | W4 => x.1.toFinset ⊆ y.1.toFinset ∧ x.2.1.toFinset ⊆ y.2.1.toFinset ∧ x.2.2 ⊆ y.2.2
+  | K1 => x.1 ⊆ y.1 ∧ x.2 ⊆ y.2
+  | K2 => x.1.toFinset ⊆ y.1.toFinset ∧ x.2.1.toFinset ⊆ y.2.1.toFinset ∧ x.2.2 ⊆ y.2.2
+  | topYukawa => x.1.toFinset ⊆ y.1.toFinset ∧ x.2 ⊆ y.2
+  | bottomYukawa => x.1.toFinset ⊆ y.1.toFinset ∧ x.2.1 ⊆ y.2.1 ∧ x.2.2 ⊆ y.2.2
+
+instance subsetDecidable : (T : PotentialTerm) → (x y : T.ChargeProfile) → Decidable (x ⊆ y)
+  | μ, _, _ => instDecidableAnd
+  | β, _, _ => instDecidableAnd
+  | Λ, _, _ => instDecidableAnd
+  | W1, _, _ => instDecidableAnd
+  | W2, _, _ => instDecidableAnd
+  | W3, _, _ => instDecidableAnd
+  | W4, _, _ => instDecidableAnd
+  | K1, _, _ => instDecidableAnd
+  | K2, _, _ => instDecidableAnd
+  | topYukawa, _, _ => instDecidableAnd
+  | bottomYukawa, _, _ => instDecidableAnd
+
+@[simp, refl]
+lemma subset_refl {T : PotentialTerm} (x : T.ChargeProfile) : x ⊆ x := by
+  fin_cases T <;> simp [Subset]
+
+@[trans]
+lemma subset_trans {T : PotentialTerm} {x y z : T.ChargeProfile} (h1 : x ⊆ y) (h2 : y ⊆ z) :
+    x ⊆ z := by
+  fin_cases T <;>
+    simp_all [Subset]
+
+
+/-!
+
+## The charges associated with the potential terms
+
+-/
+
+/-- The U(1) charges of each potential term given an element of the corresponding `ChargeProfile`.
+  For example, for the term `𝛽ᵢ 5̄Mⁱ5Hu` and `Q5 = {0, 2}` and `qHu = 3` then
+  the charges of this term would be `{-3, -1}`. -/
+def charges : {T : PotentialTerm} → T.ChargeProfile → Multiset ℤ
+  | μ, (qHd, qHu) => (qHd.toFinset.product <| qHu.toFinset).val.map (fun x => x.1 - x.2)
+  | β, (qHu, Q5) => (qHu.toFinset.product <| Q5).val.map (fun x => - x.1 + x.2)
+  | Λ, (Q5, Q10) => (Q5.product <| Q5.product <| Q10).val.map (fun x => x.1 + x.2.1 + x.2.2)
+  | W1, (Q5, Q10) => (Q5.product <| Q10.product <| Q10.product <| Q10).val.map
+    (fun x => x.1 + x.2.1 + x.2.2.1 + x.2.2.2)
+  | W2, (qHd, Q10) => (qHd.toFinset.product <| Q10.product <| Q10.product <| Q10).val.map
+    (fun x => x.1 + x.2.1 + x.2.2.1 + x.2.2.2)
+  | W3, (qHu, Q5) => (qHu.toFinset.product <| Q5.product <| Q5).val.map
+    (fun x => -x.1 - x.1 + x.2.1 + x.2.2)
+  | W4, (qHd, qHu, Q5) => (qHd.toFinset.product <| qHu.toFinset.product <| Q5).val.map
+    (fun x => x.1 - x.2.1 - x.2.1 + x.2.2)
+  | K1, (Q5, Q10) => (Q5.product <| Q10.product <| Q10).val.map
+    (fun x => - x.1 + x.2.1 + x.2.2)
+  | K2, (qHd, qHu, Q10) => (qHd.toFinset.product <| qHu.toFinset.product <| Q10).val.map
+    (fun x => x.1 + x.2.1 + x.2.2)
+  | topYukawa, (qHu, Q10) => (qHu.toFinset.product <| Q10.product <| Q10).val.map
+    (fun x => -x.1 + x.2.1 + x.2.2)
+  | bottomYukawa, (qHd, Q5, Q10) => (qHd.toFinset.product <| Q5.product <| Q10).val.map
+    (fun x => x.1 + x.2.1 + x.2.2)
+
+lemma charges_of_subset {T : PotentialTerm} {x y : T.ChargeProfile} (h : x ⊆ y) :
+    charges x ⊆ charges y := by
+  match T, x, y with
+  | μ, (qHd, qHu), (qHd', qHu') =>
+    simp only [charges, Finset.product_eq_sprod]
+    simp only [Subset] at h
+    apply Multiset.map_subset_map
+    refine Multiset.subset_iff.mpr ?_
+    intro (q1, q2) h'
+    rw [← Multiset.mem_toFinset, Finset.val_toFinset, Finset.mem_product] at ⊢ h'
+    exact ⟨h.1 h'.1, h.2 h'.2⟩
+  | β, (qHu, Q5), (qHu', Q5') =>
+    simp only [charges, Finset.product_eq_sprod]
+    simp only [Subset, instHasSubset] at h
+    apply Multiset.map_subset_map
+    refine Multiset.subset_iff.mpr ?_
+    intro (q1, q2) h'
+    rw [← Multiset.mem_toFinset, Finset.val_toFinset, Finset.mem_product] at ⊢ h'
+    exact ⟨h.1 h'.1, h.2 h'.2⟩
+  | Λ, (Q5, Q10), (Q5', Q10') =>
+    simp only [charges, Finset.product_eq_sprod]
+    simp only [Subset, instHasSubset] at h
+    apply Multiset.map_subset_map
+    refine Multiset.subset_iff.mpr ?_
+    intro (q1, q2, q3) h'
+    rw [← Multiset.mem_toFinset, Finset.val_toFinset, Finset.mem_product,
+      Finset.mem_product] at ⊢ h'
+    exact ⟨h.1 h'.1, h.1 h'.2.1, h.2 h'.2.2⟩
+  | W1, (Q5, Q10), (Q5', Q10') =>
+    simp only [charges, Finset.product_eq_sprod]
+    simp only [Subset, instHasSubset] at h
+    apply Multiset.map_subset_map
+    refine Multiset.subset_iff.mpr ?_
+    intro (q1, q2, q3, q4) h'
+    rw [← Multiset.mem_toFinset, Finset.val_toFinset, Finset.mem_product,
+      Finset.mem_product, Finset.mem_product] at ⊢ h'
+    exact ⟨h.1 h'.1, h.2 h'.2.1, h.2 h'.2.2.1, h.2 h'.2.2.2⟩
+  | W2, (qHd, Q10), (qHd', Q10') =>
+    simp only [charges, Finset.product_eq_sprod]
+    simp only [Subset, instHasSubset] at h
+    apply Multiset.map_subset_map
+    refine Multiset.subset_iff.mpr ?_
+    intro (q1, q2, q3, q4) h'
+    rw [← Multiset.mem_toFinset, Finset.val_toFinset, Finset.mem_product,
+      Finset.mem_product, Finset.mem_product] at ⊢ h'
+    exact ⟨h.1 h'.1, h.2 h'.2.1, h.2 h'.2.2.1, h.2 h'.2.2.2⟩
+  | W3, (qHu, Q5), (qHu', Q5') =>
+    simp only [charges, Finset.product_eq_sprod]
+    simp only [Subset, instHasSubset] at h
+    apply Multiset.map_subset_map
+    refine Multiset.subset_iff.mpr ?_
+    intro (q1, q2, q3) h'
+    rw [← Multiset.mem_toFinset, Finset.val_toFinset, Finset.mem_product,
+      Finset.mem_product] at ⊢ h'
+    exact ⟨h.1 h'.1, h.2 h'.2.1, h.2 h'.2.2⟩
+  | W4, (qHd, qHu, Q5), (qHd', qHu', Q5') =>
+    simp only [charges, Finset.product_eq_sprod]
+    simp only [Subset, instHasSubset] at h
+    apply Multiset.map_subset_map
+    refine Multiset.subset_iff.mpr ?_
+    intro (q1, q2, q3) h'
+    rw [← Multiset.mem_toFinset, Finset.val_toFinset, Finset.mem_product,
+      Finset.mem_product] at ⊢ h'
+    exact ⟨h.1 h'.1, h.2.1 h'.2.1, h.2.2 h'.2.2⟩
+  | K1, (Q5, Q10), (Q5', Q10') =>
+    simp only [charges, Finset.product_eq_sprod]
+    simp only [Subset, instHasSubset] at h
+    apply Multiset.map_subset_map
+    refine Multiset.subset_iff.mpr ?_
+    intro (q1, q2, q3) h'
+    rw [← Multiset.mem_toFinset, Finset.val_toFinset, Finset.mem_product,
+      Finset.mem_product] at ⊢ h'
+    exact ⟨h.1 h'.1, h.2 h'.2.1, h.2 h'.2.2⟩
+  | K2, (qHd, qHu, Q10), (qHd', qHu', Q10') =>
+    simp only [charges, Finset.product_eq_sprod]
+    simp only [Subset, instHasSubset] at h
+    apply Multiset.map_subset_map
+    refine Multiset.subset_iff.mpr ?_
+    intro (q1, q2, q3) h'
+    rw [← Multiset.mem_toFinset, Finset.val_toFinset, Finset.mem_product,
+      Finset.mem_product] at ⊢ h'
+    exact ⟨h.1 h'.1, h.2.1 h'.2.1, h.2.2 h'.2.2⟩
+  | topYukawa, (qHu, Q10), (qHu', Q10') =>
+    simp only [charges, Finset.product_eq_sprod]
+    simp only [Subset, instHasSubset] at h
+    apply Multiset.map_subset_map
+    refine Multiset.subset_iff.mpr ?_
+    intro (q1, q2, q3) h'
+    rw [← Multiset.mem_toFinset, Finset.val_toFinset, Finset.mem_product,
+      Finset.mem_product] at ⊢ h'
+    exact ⟨h.1 h'.1, h.2 h'.2.1, h.2 h'.2.2⟩
+  | bottomYukawa, (qHd, Q5, Q10), (qHd', Q5', Q10') =>
+    simp only [charges, Finset.product_eq_sprod]
+    simp only [Subset, instHasSubset] at h
+    apply Multiset.map_subset_map
+    refine Multiset.subset_iff.mpr ?_
+    intro (q1, q2, q3) h'
+    rw [← Multiset.mem_toFinset, Finset.val_toFinset, Finset.mem_product,
+      Finset.mem_product] at ⊢ h'
+    exact ⟨h.1 h'.1, h.2.1 h'.2.1, h.2.2 h'.2.2⟩
+
+/-- Given a `I : CodimensionOneConfig`, and a potential term `PotentialTerm`, the
+  possible finite set of elements of `T.ChargeProfile` which orginate from charges allowed by `I`. -/
+def chargeSubsetFull (I : CodimensionOneConfig) (T : PotentialTerm) : Finset T.ChargeProfile :=
+  let SqHd := {none} ∪ I.allowedBarFiveCharges.map ⟨Option.some, Option.some_injective ℤ⟩
+  let SqHu := {none} ∪ I.allowedBarFiveCharges.map ⟨Option.some, Option.some_injective ℤ⟩
+  let SQ5 := I.allowedBarFiveCharges.powerset
+  let SQ10 := I.allowedTenCharges.powerset
+  match T with
+  | μ => SqHd.product SqHu
+  | K2 => SqHd.product (SqHu.product SQ10)
+  | K1 => SQ5.product SQ10
+  | W4 => SqHd.product (SqHu.product SQ5)
+  | W3 => SqHu.product SQ5
+  | W2 => SqHd.product SQ10
+  | W1 => SQ5.product SQ10
+  | Λ => SQ5.product SQ10
+  | β => SqHu.product SQ5
+  | topYukawa => SqHu.product SQ10
+  | bottomYukawa => SqHd.product (SQ5.product SQ10)
+
+/-!
+
+## Excluded terms based on `U(1)` charges
+
+The terms in the potential can be excluded based on the presences of `U(1)` charges
+they carry.
+
+-/
+
+/-- Given a potential term `T` with an element of it's associated `ChargeProfile`, the proposition
+  corresonding to there been no `zero` in the charges of that term. That is to say, it is excluded
+  by the `U(1)` charges.
+
+  For example, for the term `𝛽ᵢ 5̄Mⁱ5Hu` and `Q5 = {0, 2}` and `qHu = 3`
+  the charges of this term are `{-3, -1}`, and this is excluded by the `U(1)` charges.
+  Thus `IsExcluded β (3, {0, 2})` would be `true`.
+  -/
+def IsExcluded {T : PotentialTerm} (x : T.ChargeProfile) : Prop :=
+  0 ∉ charges x
+
+/-!
+
+### Decidability of `IsExcluded`
+
+-/
+
+/-- The decidability of `IsExcluded` for the potential terms. -/
+instance : (T : PotentialTerm) → DecidablePred (IsExcluded (T := T))
+  | μ => fun _ => instDecidableNot
+  | β => fun _ => instDecidableNot
+  | Λ => fun _ => instDecidableNot
+  | W1 => fun _ => instDecidableNot
+  | W2 => fun _ => instDecidableNot
+  | W3 => fun _ => instDecidableNot
+  | W4 => fun _ => instDecidableNot
+  | K1 => fun _ =>instDecidableNot
+  | K2 => fun _ => instDecidableNot
+  | topYukawa => fun _ => instDecidableNot
+  | bottomYukawa => fun _ => instDecidableNot
+
+/-!
+
+## Present terms based on `U(1)` charges
+
+The terms in the potential can be present based on the presences of `U(1)` charges
+they carry.
+
+Of particular intrest is the presence of the top Yukawa term.
+
+-/
+
+/-- Given a potential term `T` with an element of it's associated `ChargeProfile`, the proposition
+  corresonding to there been `zero` in the charges of that term. That is to say, it is present
+  by the `U(1)` charges.
+
+  For example, for the term `𝛽ᵢ 5̄Mⁱ5Hu` and `Q5 = {0, 2}` and `qHu = 2`
+  the charges of this term are `{-2, 0}`, and this is excluded by the `U(1)` charges.
+  Thus `IsPresent β (3, {0, 2})` would be `true`.
+-/
+def IsPresent (T : PotentialTerm) (x : T.ChargeProfile) : Prop :=
+  0 ∈ x.charges
+
+lemma not_isExcluded_iff_isPresent : (T : PotentialTerm) → (x : T.ChargeProfile) →
+    ¬ x.IsExcluded ↔ x.IsPresent
+  | μ => fun (qHd, qHu) => by simp [IsExcluded, IsPresent]
+  | β => fun (qHu, Q5) => by simp [IsExcluded, IsPresent]
+  | Λ => fun (Q5, Q10) => by simp [IsExcluded, IsPresent]
+  | W1 => fun (Q5, Q10) => by simp [IsExcluded, IsPresent]
+  | W2 => fun (qHd, Q10) => by simp [IsExcluded, IsPresent]
+  | W3 => fun (qHu, Q5) => by simp [IsExcluded, IsPresent]
+  | W4 => fun (qHd, qHu, Q5) => by simp [IsExcluded, IsPresent]
+  | K1 => fun (Q5, Q10) => by simp [IsExcluded, IsPresent]
+  | K2 => fun (qHd, qHu, Q10) => by simp [IsExcluded, IsPresent]
+  | topYukawa => fun (qHu, Q10) => by simp [IsExcluded, IsPresent]
+  | bottomYukawa => fun (qHd, Q5, Q10) => by simp [IsExcluded, IsPresent]
+
+/-- The decidability of `IsPresent` for the potential terms. -/
+instance (T : PotentialTerm) : DecidablePred (IsPresent (T := T)) :=
+  fun _ => Multiset.decidableMem _ _
+
+lemma isPresent_of_subset {T : PotentialTerm} {y x : T.ChargeProfile}
+    (h : y ⊆ x) (hy : y.IsPresent) : x.IsPresent := charges_of_subset h hy
+
+/-!
+
+## Powersets of charge profiles
+
+-/
+
+/-- The powerset of `x : Option ℤ` defined as `{none}` if `x` is `none`
+  and `{none, some y}` is `x` is `some y`.-/
+def _root_.Option.powerset (x : Option ℤ) : Finset (Option ℤ) :=
+  match x with
+  | none => {none}
+  | some x => {none, some x}
+
+@[simp]
+lemma _root_.Option.mem_powerset_iff {x : Option ℤ} (y : Option ℤ) :
+    y ∈ x.powerset ↔ y.toFinset ⊆ x.toFinset :=
+  match x, y with
+  | none, none => by
+    simp [Option.powerset]
+  | none, some _ => by
+    simp [Option.powerset]
+  | some _, none => by
+    simp [Option.powerset]
+  | some _, some _ => by
+    simp [Option.powerset]
+
+/-- The powerset of a charge profile. Given a charge profile `x : T.ChargeProfile`
+  it's powerset is the finite set of all `T.ChargeProfile` which are subsets of `x`. -/
+def powerset {T : PotentialTerm} (x : T.ChargeProfile) : Finset T.ChargeProfile :=
+  match T, x with
+  | μ, (qHd, qHu) => qHd.powerset.product qHu.powerset
+  | β, (qHu, Q5) => qHu.powerset.product Q5.powerset
+  | Λ, (Q5, Q10) => Q5.powerset.product Q10.powerset
+  | W1, (Q5, Q10) => Q5.powerset.product Q10.powerset
+  | W2, (qHd, Q10) => qHd.powerset.product Q10.powerset
+  | W3, (qHu, Q5) => qHu.powerset.product Q5.powerset
+  | W4, (qHd, qHu, Q5) => qHd.powerset.product (qHu.powerset.product Q5.powerset)
+  | K1, (Q5, Q10) => Q5.powerset.product Q10.powerset
+  | K2, (qHd, qHu, Q10) => qHd.powerset.product (qHu.powerset.product Q10.powerset)
+  | topYukawa, (qHu, Q10) => qHu.powerset.product Q10.powerset
+  | bottomYukawa, (qHd, Q5, Q10) => qHd.powerset.product (Q5.powerset.product Q10.powerset)
+
+lemma subset_of_iff_mem_powerset {T : PotentialTerm} {x y : T.ChargeProfile} :
+    x ⊆ y ↔ x ∈ powerset y := by
+  fin_cases T
+  all_goals
+    cases x
+    cases y
+    simp only [powerset, Finset.product_eq_sprod]
+    rw [Finset.mem_product]
+    simp_all [Subset]
+
+@[simp]
+lemma self_mem_powerset {T : PotentialTerm} (x : T.ChargeProfile) :
+    x ∈ powerset x := by
+  rw [← subset_of_iff_mem_powerset]
+
+end ChargeProfile
+
+end PotentialTerm
+
+end SU5U1
+
+end FTheory
