PhysLean/StringTheory/FTheory/SU5U1/Potential/ChargeProfile/Irreducible/Basic.lean
@@ -1,0 +1,54 @@
+/-
+Copyright (c) 2025 Joseph Tooby-Smith. All rights reserved.
+Released under Apache 2.0 license as described in the file LICENSE.
+Authors: Joseph Tooby-Smith
+-/
+import PhysLean.StringTheory.FTheory.SU5U1.Potential.ChargeProfile.Basic
+/-!
+
+# Irreducible Charge Profiles
+
+An irreducible charge profile is a charge profile that allows it's potential term,
+but for which no other member of its powerset allows the potential term.
+
+## Related PRs
+
+- See #562 for a first version of code related to charge profiles.
+
+-/
+namespace FTheory
+
+namespace SU5U1
+
+variable {I : CodimensionOneConfig}
+namespace PotentialTerm
+
+namespace ChargeProfile
+
+/-- For a potential term `T`, an `x : T.ChargeProfile` is said to be irreducible if
+  it allows the term `T`, and no other member of it's powerset allows `T`. -/
+def IsIrreducible {T : PotentialTerm} (x : T.ChargeProfile) : Prop :=
+  ∀ y ∈ powerset x, y = x ↔ IsPresent T y
+
+instance {T : PotentialTerm} (x : T.ChargeProfile) : Decidable x.IsIrreducible :=
+  inferInstanceAs (Decidable (∀ y ∈ powerset x, y = x ↔ IsPresent T y))
+
+lemma isPresent_of_isIrreducible {T : PotentialTerm} {x : T.ChargeProfile} (h : IsIrreducible x) :
+    IsPresent T x := by
+  simp [IsIrreducible] at h
+  simpa using h x (self_mem_powerset x)
+
+lemma isPresent_of_has_isIrreducible_subset {T : PotentialTerm} {x : T.ChargeProfile}
+    (hx : ∃ y ∈ powerset x, IsIrreducible y) : IsPresent T x := by
+  obtain ⟨y, hy⟩ := hx
+  rw [← subset_of_iff_mem_powerset] at hy
+  apply isPresent_of_subset hy.1
+  exact isPresent_of_isIrreducible hy.2
+
+end ChargeProfile
+
+end PotentialTerm
+
+end SU5U1
+
+end FTheory
